Anotate the spec

AwsCryptographicMaterialProviders/dafny/AwsCryptographyKeyStore/src/GetKeys.dfy
@@ -64,73 +64,22 @@ module GetKeys {
               && Structure.BRANCH_KEY_ACTIVE_VERSION_FIELD in activeItem
 
               && KMSKeystoreOperations.AttemptKmsOperation?(kmsConfiguration, Structure.ToBranchKeyContext(activeItem, logicalKeyStoreName))
+              && |kmsClient.History.Decrypt| == |old(kmsClient.History.Decrypt)| + 1
 
               //= aws-encryption-sdk-specification/framework/branch-key-store.md#getactivebranchkey
               //= type=implication
               //# The operation MUST decrypt the branch key according to the [AWS KMS Branch Key Decryption](#aws-kms-branch-key-decryption) section.
+              && AwsKmsBranchKeyDecryption?(
+                   Seq.Last(ddbClient.History.GetItem),
+                   Seq.Last(kmsClient.History.Decrypt),
+                   kmsClient,
+                   ddbClient,
+                   kmsConfiguration,
+                   grantTokens,
+                   logicalKeyStoreName
+                 )
 
               && var versionEncryptionContext := Structure.ToBranchKeyContext(activeItem, logicalKeyStoreName);
-
-              //= aws-encryption-sdk-specification/framework/branch-key-store.md#aws-kms-branch-key-decryption
-              //= type=implication
-              //# Every key in the constructed [encryption context](#encryption-context)
-              //# except `tableName`
-              //# MUST exist as a string attribute in the AWS DDB response item.
-              && versionEncryptionContext.Keys - {Structure.TABLE_FIELD} < activeItem.Keys
-
-              //= aws-encryption-sdk-specification/framework/branch-key-store.md#aws-kms-branch-key-decryption
-              //= type=implication
-              //# Every value in the constructed [encryption context](#encryption-context)
-              //# except the logical table name
-              //# MUST equal the value with the same key in the AWS DDB response item.
-              && (forall k <- versionEncryptionContext.Keys - {Structure.TABLE_FIELD}
-                    :: match k
-                       case HIERARCHY_VERSION => versionEncryptionContext[Structure.HIERARCHY_VERSION] == activeItem[Structure.HIERARCHY_VERSION].N
-                       case _ => versionEncryptionContext[k] == activeItem[k].S)
-
-              //= aws-encryption-sdk-specification/framework/branch-key-store.md#aws-kms-branch-key-decryption
-              //= type=implication
-              //# The key `enc` MUST NOT exist in the constructed [encryption context](#encryption-context).
-              && Structure.BRANCH_KEY_FIELD !in  versionEncryptionContext
-
-              //= aws-encryption-sdk-specification/framework/branch-key-store.md#aws-kms-branch-key-decryption
-              //= type=implication
-              //# The operation MUST use the configured `KMS SDK Client` to decrypt the value of the branch key field.
-              && |kmsClient.History.Decrypt| == |old(kmsClient.History.Decrypt)| + 1
-
-              //= aws-encryption-sdk-specification/framework/branch-key-store.md#aws-kms-branch-key-decryption
-              //= type=implication
-              //# When calling [AWS KMS Decrypt](https://docs.aws.amazon.com/kms/latest/APIReference/API_Decrypt.html),
-              //# the keystore operation MUST call with a request constructed as follows:
-              && var decryptRequest := Seq.Last(kmsClient.History.Decrypt).input;
-
-              //= aws-encryption-sdk-specification/framework/branch-key-store.md#aws-kms-branch-key-decryption
-              //= type=implication
-              //# - `KeyId` MUST be the configured `AWS KMS Key ARN` in the [AWS KMS Configuration](#aws-kms-configuration) for this keystore
-              && decryptRequest.KeyId == Some(kmsConfiguration.kmsKeyArn)
-
-              //= aws-encryption-sdk-specification/framework/branch-key-store.md#aws-kms-branch-key-decryption
-              //= type=implication
-              //# - `CiphertextBlob` MUST be the `enc` attribute value on the AWS DDB response item
-              && decryptRequest.CiphertextBlob == activeItem[Structure.BRANCH_KEY_FIELD].B
-
-              //= aws-encryption-sdk-specification/framework/branch-key-store.md#aws-kms-branch-key-decryption
-              //= type=implication
-              //# Every attribute except for `enc` on the AWS DDB response item
-              //# MUST be authenticated in the decryption of `enc`
-
-              //= aws-encryption-sdk-specification/framework/branch-key-store.md#aws-kms-branch-key-decryption
-              //= type=implication
-              //# - `EncryptionContext` MUST be the [encryption context](#encryption-context) constructed above
-              && decryptRequest.EncryptionContext == Some(versionEncryptionContext)
-
-              //= aws-encryption-sdk-specification/framework/branch-key-store.md#aws-kms-branch-key-decryption
-              //= type=implication
-              //# - `GrantTokens` MUST be this keystore's [grant tokens](https://docs.aws.amazon.com/kms/latest/developerguide/concepts.html#grant_token).
-              && decryptRequest.GrantTokens == Some(grantTokens)
-
-              && Seq.Last(kmsClient.History.Decrypt).output.Success?
-              && Seq.Last(kmsClient.History.Decrypt).output.value.Plaintext.Some?
               && var decryptResponse := Seq.Last(kmsClient.History.Decrypt).output.value;
 
               && Structure.ToBranchKeyMaterials(versionEncryptionContext, decryptResponse.Plaintext.value).Success?
@@ -217,8 +166,6 @@ module GetKeys {
     modifies ddbClient.Modifies, kmsClient.Modifies
     ensures ddbClient.ValidState() && kmsClient.ValidState()
 
-
-
     ensures
       //= aws-encryption-sdk-specification/framework/branch-key-store.md#getbranchkeyversion
       //= type=implication
@@ -247,73 +194,22 @@ module GetKeys {
               && Structure.BRANCH_KEY_TYPE_PREFIX < versionItem[Structure.TYPE_FIELD].S
 
               && KMSKeystoreOperations.AttemptKmsOperation?(kmsConfiguration, Structure.ToBranchKeyContext(versionItem, logicalKeyStoreName))
+              && |kmsClient.History.Decrypt| == |old(kmsClient.History.Decrypt)| + 1
 
               //= aws-encryption-sdk-specification/framework/branch-key-store.md#getbranchkeyversion
               //= type=implication
               //# The operation MUST decrypt the branch key according to the [AWS KMS Branch Key Decryption](#aws-kms-branch-key-decryption) section.
+              && AwsKmsBranchKeyDecryption?(
+                   Seq.Last(ddbClient.History.GetItem),
+                   Seq.Last(kmsClient.History.Decrypt),
+                   kmsClient,
+                   ddbClient,
+                   kmsConfiguration,
+                   grantTokens,
+                   logicalKeyStoreName
+                 )
 
               && var versionEncryptionContext := Structure.ToBranchKeyContext(versionItem, logicalKeyStoreName);
-
-              //= aws-encryption-sdk-specification/framework/branch-key-store.md#aws-kms-branch-key-decryption
-              //= type=implication
-              //# Every key in the constructed [encryption context](#encryption-context)
-              //# except `tableName`
-              //# MUST exist as a string attribute in the AWS DDB response item.
-              && versionEncryptionContext.Keys - {Structure.TABLE_FIELD} < versionItem.Keys
-
-              //= aws-encryption-sdk-specification/framework/branch-key-store.md#aws-kms-branch-key-decryption
-              //= type=implication
-              //# Every value in the constructed [encryption context](#encryption-context)
-              //# except the logical table name
-              //# MUST equal the value with the same key in the AWS DDB response item.
-              && (forall k <- versionEncryptionContext.Keys - {Structure.TABLE_FIELD}
-                    :: match k
-                       case HIERARCHY_VERSION => versionEncryptionContext[Structure.HIERARCHY_VERSION] == versionItem[Structure.HIERARCHY_VERSION].N
-                       case _ => versionEncryptionContext[k] == versionItem[k].S)
-
-              //= aws-encryption-sdk-specification/framework/branch-key-store.md#aws-kms-branch-key-decryption
-              //= type=implication
-              //# The key `enc` MUST NOT exist in the constructed [encryption context](#encryption-context).
-              && Structure.BRANCH_KEY_FIELD !in  versionEncryptionContext
-
-              //= aws-encryption-sdk-specification/framework/branch-key-store.md#aws-kms-branch-key-decryption
-              //= type=implication
-              //# The operation MUST use the configured `KMS SDK Client` to decrypt the value of the branch key field.
-              && |kmsClient.History.Decrypt| == |old(kmsClient.History.Decrypt)| + 1
-
-              //= aws-encryption-sdk-specification/framework/branch-key-store.md#aws-kms-branch-key-decryption
-              //= type=implication
-              //# When calling [AWS KMS Decrypt](https://docs.aws.amazon.com/kms/latest/APIReference/API_Decrypt.html),
-              //# the keystore operation MUST call with a request constructed as follows:
-              && var decryptRequest := Seq.Last(kmsClient.History.Decrypt).input;
-
-              //= aws-encryption-sdk-specification/framework/branch-key-store.md#aws-kms-branch-key-decryption
-              //= type=implication
-              //# - `KeyId` MUST be the configured `AWS KMS Key ARN` in the [AWS KMS Configuration](#aws-kms-configuration) for this keystore
-              && decryptRequest.KeyId == Some(kmsConfiguration.kmsKeyArn)
-
-              //= aws-encryption-sdk-specification/framework/branch-key-store.md#aws-kms-branch-key-decryption
-              //= type=implication
-              //# - `CiphertextBlob` MUST be the `enc` attribute value on the AWS DDB response item
-              && decryptRequest.CiphertextBlob == versionItem[Structure.BRANCH_KEY_FIELD].B
-
-              //= aws-encryption-sdk-specification/framework/branch-key-store.md#aws-kms-branch-key-decryption
-              //= type=implication
-              //# Every attribute except for `enc` on the AWS DDB response item
-              //# MUST be authenticated in the decryption of `enc`
-
-              //= aws-encryption-sdk-specification/framework/branch-key-store.md#aws-kms-branch-key-decryption
-              //= type=implication
-              //# - `EncryptionContext` MUST be the [encryption context](#encryption-context) constructed above
-              && decryptRequest.EncryptionContext == Some(versionEncryptionContext)
-
-              //= aws-encryption-sdk-specification/framework/branch-key-store.md#aws-kms-branch-key-decryption
-              //= type=implication
-              //# - `GrantTokens` MUST be this keystore's [grant tokens](https://docs.aws.amazon.com/kms/latest/developerguide/concepts.html#grant_token).
-              && decryptRequest.GrantTokens == Some(grantTokens)
-
-              && Seq.Last(kmsClient.History.Decrypt).output.Success?
-              && Seq.Last(kmsClient.History.Decrypt).output.value.Plaintext.Some?
               && var decryptResponse := Seq.Last(kmsClient.History.Decrypt).output.value;
 
               && Structure.ToBranchKeyMaterials(versionEncryptionContext, decryptResponse.Plaintext.value).Success?
@@ -322,10 +218,12 @@ module GetKeys {
               //= type=implication
               //# This GetBranchKeyVersion MUST construct [beacon key materials](./structures.md#beacon-key-materials)
               //# according to [Branch Key Materials From Authenticated Encryption Context](#branch-key-materials-from-authenticated-encryption-context).
-              && var branchKeyMaterials :=  Structure.ToBranchKeyMaterials(
-                                              versionEncryptionContext,
-                                              decryptResponse.Plaintext.value
-                                            ).value;
+              && var branchKeyMaterials := Structure
+                                           .ToBranchKeyMaterials(
+                                             versionEncryptionContext,
+                                             decryptResponse.Plaintext.value
+                                           )
+                                           .value;
 
               //= aws-encryption-sdk-specification/framework/branch-key-store.md#getbranchkeyversion
               //= type=implication
@@ -400,71 +298,82 @@ module GetKeys {
     modifies ddbClient.Modifies, kmsClient.Modifies
     ensures ddbClient.ValidState() && kmsClient.ValidState()
 
+    ensures
+      //= aws-encryption-sdk-specification/framework/branch-key-store.md#getbeaconkey
+      //= type=implication
+      //# To get a branch key from the keystore this operation MUST call AWS DDB `GetItem`
+      //# using the `branch-key-id` as the Partition Key and "beacon:ACTIVE" value as the Sort Key.
+      && |ddbClient.History.GetItem| == |old(ddbClient.History.GetItem)| + 1
+      && Seq.Last(ddbClient.History.GetItem).input.Key
+         == map[
+              Structure.BRANCH_KEY_IDENTIFIER_FIELD := DDB.AttributeValue.S(input.branchKeyIdentifier),
+              Structure.TYPE_FIELD := DDB.AttributeValue.S(Structure.BEACON_KEY_TYPE_VALUE)
+            ]
+
     ensures output.Success? ==>
               && Seq.Last(ddbClient.History.GetItem).output.Success?
               && Seq.Last(ddbClient.History.GetItem).output.value.Item.Some?
               && var versionItem := Seq.Last(ddbClient.History.GetItem).output.value.Item.value;
 
-
+              //= aws-encryption-sdk-specification/framework/branch-key-store.md#getbeaconkey
+              //= type=implication
+              //# The AWS DDB response MUST contain the fields defined in the [branch keystore record format](#record-format).
               && Structure.BranchKeyItem?(versionItem)
               && versionItem[Structure.HIERARCHY_VERSION].N?
               && Structure.BRANCH_KEY_ACTIVE_VERSION_FIELD !in versionItem
               && versionItem[Structure.TYPE_FIELD].S == Structure.BEACON_KEY_TYPE_VALUE
 
               && KMSKeystoreOperations.AttemptKmsOperation?(kmsConfiguration, Structure.ToBranchKeyContext(versionItem, logicalKeyStoreName))
-
-
-              && var versionEncryptionContext := Structure.ToBranchKeyContext(versionItem, logicalKeyStoreName);
-
-              && versionEncryptionContext.Keys - {Structure.TABLE_FIELD} < versionItem.Keys
-
-              && (forall k <- versionEncryptionContext.Keys - {Structure.TABLE_FIELD}
-                    :: match k
-                       case HIERARCHY_VERSION => versionEncryptionContext[Structure.HIERARCHY_VERSION] == versionItem[Structure.HIERARCHY_VERSION].N
-                       case _ => versionEncryptionContext[k] == versionItem[k].S)
-
-              && Structure.BRANCH_KEY_FIELD !in  versionEncryptionContext
-
               && |kmsClient.History.Decrypt| == |old(kmsClient.History.Decrypt)| + 1
 
-              && var decryptRequest := Seq.Last(kmsClient.History.Decrypt).input;
+              //= aws-encryption-sdk-specification/framework/branch-key-store.md#getbeaconkey
+              //= type=implication
+              //# The operation MUST decrypt the beacon key according to the [AWS KMS Branch Key Decryption](#aws-kms-branch-key-decryption) section.
+              && AwsKmsBranchKeyDecryption?(
+                   Seq.Last(ddbClient.History.GetItem),
+                   Seq.Last(kmsClient.History.Decrypt),
+                   kmsClient,
+                   ddbClient,
+                   kmsConfiguration,
+                   grantTokens,
+                   logicalKeyStoreName
+                 )
 
-
-              && decryptRequest.KeyId == Some(kmsConfiguration.kmsKeyArn)
-
-              && decryptRequest.CiphertextBlob == versionItem[Structure.BRANCH_KEY_FIELD].B
-
-              && decryptRequest.EncryptionContext == Some(versionEncryptionContext)
-
-
-              && decryptRequest.GrantTokens == Some(grantTokens)
-
-              && Seq.Last(kmsClient.History.Decrypt).output.Success?
-              && Seq.Last(kmsClient.History.Decrypt).output.value.Plaintext.Some?
+              && var versionEncryptionContext := Structure.ToBranchKeyContext(versionItem, logicalKeyStoreName);
               && var decryptResponse := Seq.Last(kmsClient.History.Decrypt).output.value;
 
               && Structure.ToBeaconKeyMaterials(versionEncryptionContext, decryptResponse.Plaintext.value).Success?
 
+              //= aws-encryption-sdk-specification/framework/branch-key-store.md#getbeaconkey
+              //= type=implication
+              //# This GetBeaconKey MUST construct [beacon key materials](./structures.md#beacon-key-materials) from the decrypted branch key material
+              //# and the `branchKeyId` from the returned `branch-key-id` field.
+              && var beaconKeyMaterials := Structure.ToBeaconKeyMaterials(
+                                             versionEncryptionContext,
+                                             decryptResponse.Plaintext.value
+                                           ).value;
 
-              && var beaconKeyMaterials :=  Structure.ToBeaconKeyMaterials(
-                                              versionEncryptionContext,
-                                              decryptResponse.Plaintext.value
-                                            ).value;
-
-
+              //= aws-encryption-sdk-specification/framework/branch-key-store.md#getbeaconkey
+              //= type=implication
+              //# This operation MUST return the constructed [beacon key materials](./structures.md#beacon-key-materials).
               && output.value.beaconKeyMaterials == beaconKeyMaterials
 
               && output.value.beaconKeyMaterials.beaconKeyIdentifier == input.branchKeyIdentifier
 
     ensures
 
+      //= aws-encryption-sdk-specification/framework/branch-key-store.md#getbeaconkey
+      //= type=implication
+      //# If the record does not contain the defined fields, this operation MUST fail.
       || (&& |ddbClient.History.GetItem| == |old(ddbClient.History.GetItem)| + 1
           && Seq.Last(ddbClient.History.GetItem).output.Success?
           && Seq.Last(ddbClient.History.GetItem).output.value.Item.Some?
           && !Structure.BeaconKeyItem?(Seq.Last(ddbClient.History.GetItem).output.value.Item.value)
           ==> output.Failure?)
 
-
+      //= aws-encryption-sdk-specification/framework/branch-key-store.md#getbeaconkey
+      //= type=implication
+      //# If the beacon key fails to decrypt, this operation MUST fail.
       || (&& |kmsClient.History.Decrypt| == |old(kmsClient.History.Decrypt)| + 1
           && Seq.Last(kmsClient.History.Decrypt).output.Failure?
           ==> output.Failure?)
@@ -474,7 +383,6 @@ module GetKeys {
       tableName,
       ddbClient
     );
-    assert Seq.Last(ddbClient.History.GetItem).output.Success?;
 
     var encryptionContext := Structure.ToBranchKeyContext(branchKeyItem, logicalKeyStoreName);
 
@@ -491,8 +399,6 @@ module GetKeys {
       kmsClient
     );
 
-    assert Seq.Last(ddbClient.History.GetItem).output.Success?;
-
     var branchKeyMaterials :- Structure.ToBeaconKeyMaterials(
       encryptionContext,
       branchKey.Plaintext.value
@@ -502,5 +408,95 @@ module GetKeys {
                      beaconKeyMaterials := branchKeyMaterials
                    ));
   }
+
+
+  predicate AwsKmsBranchKeyDecryption?(
+    getItemHistory: DDB.DafnyCallEvent<DDB.GetItemInput, Result<DDB.GetItemOutput, DDB.Error>>,
+    decryptHistory: KMS.DafnyCallEvent<KMS.DecryptRequest, Result<KMS.DecryptResponse, KMS.Error>>,
+    kmsClient: KMS.IKMSClient,
+    ddbClient: DDB.IDynamoDBClient,
+    kmsConfiguration: Types.KMSConfiguration,
+    grantTokens: KMS.GrantTokenList,
+    logicalKeyStoreName: string
+  )
+    reads kmsClient.History
+    reads ddbClient.History
+
+    requires
+      && getItemHistory.output.Success?
+      && getItemHistory.output.value.Item.Some?
+      && Structure.BranchKeyItem?(getItemHistory.output.value.Item.value)
+         // && Structure.BRANCH_KEY_ACTIVE_VERSION_FIELD !in getItemHistory.output.value.Item.value
+         // // && Structure.BRANCH_KEY_TYPE_PREFIX < getItemHistory.output.value.Item.value[Structure.TYPE_FIELD].S
+      && getItemHistory.output.Success?
+      && getItemHistory.output.value.Item.Some?
+  {
+
+    var versionItem := getItemHistory.output.value.Item.value;
+    var versionEncryptionContext := Structure.ToBranchKeyContext(versionItem, logicalKeyStoreName);
+
+    //= aws-encryption-sdk-specification/framework/branch-key-store.md#aws-kms-branch-key-decryption
+    //= type=implication
+    //# Every key in the constructed [encryption context](#encryption-context)
+    //# except `tableName`
+    //# MUST exist as a string attribute in the AWS DDB response item.
+    && versionEncryptionContext.Keys - {Structure.TABLE_FIELD} < versionItem.Keys
+
+    //= aws-encryption-sdk-specification/framework/branch-key-store.md#aws-kms-branch-key-decryption
+    //= type=implication
+    //# Every value in the constructed [encryption context](#encryption-context)
+    //# except the logical table name
+    //# MUST equal the value with the same key in the AWS DDB response item.
+    && (forall k <- versionEncryptionContext.Keys - {Structure.TABLE_FIELD}
+          :: match k
+             case HIERARCHY_VERSION => versionEncryptionContext[Structure.HIERARCHY_VERSION] == versionItem[Structure.HIERARCHY_VERSION].N
+             case _ => versionEncryptionContext[k] == versionItem[k].S)
+
+    //= aws-encryption-sdk-specification/framework/branch-key-store.md#aws-kms-branch-key-decryption
+    //= type=implication
+    //# The key `enc` MUST NOT exist in the constructed [encryption context](#encryption-context).
+    && Structure.BRANCH_KEY_FIELD !in  versionEncryptionContext
+
+    //= aws-encryption-sdk-specification/framework/branch-key-store.md#aws-kms-branch-key-decryption
+    //= type=implication
+    //# The operation MUST use the configured `KMS SDK Client` to decrypt the value of the branch key field.
+    // && |kmsClient.History.Decrypt| == |old(kmsClient.History.Decrypt)| + 1
+
+    //= aws-encryption-sdk-specification/framework/branch-key-store.md#aws-kms-branch-key-decryption
+    //= type=implication
+    //# When calling [AWS KMS Decrypt](https://docs.aws.amazon.com/kms/latest/APIReference/API_Decrypt.html),
+    //# the keystore operation MUST call with a request constructed as follows:
+    && var decryptRequest := decryptHistory.input;
+
+    //= aws-encryption-sdk-specification/framework/branch-key-store.md#aws-kms-branch-key-decryption
+    //= type=implication
+    //# - `KeyId` MUST be the configured `AWS KMS Key ARN` in the [AWS KMS Configuration](#aws-kms-configuration) for this keystore
+    && decryptRequest.KeyId == Some(kmsConfiguration.kmsKeyArn)
+
+    //= aws-encryption-sdk-specification/framework/branch-key-store.md#aws-kms-branch-key-decryption
+    //= type=implication
+    //# - `CiphertextBlob` MUST be the `enc` attribute value on the AWS DDB response item
+    && decryptRequest.CiphertextBlob == versionItem[Structure.BRANCH_KEY_FIELD].B
+
+    //= aws-encryption-sdk-specification/framework/branch-key-store.md#aws-kms-branch-key-decryption
+    //= type=implication
+    //# Every attribute except for `enc` on the AWS DDB response item
+    //# MUST be authenticated in the decryption of `enc`
+
+    //= aws-encryption-sdk-specification/framework/branch-key-store.md#aws-kms-branch-key-decryption
+    //= type=implication
+    //# - `EncryptionContext` MUST be the [encryption context](#encryption-context) constructed above
+    && decryptRequest.EncryptionContext == Some(versionEncryptionContext)
+
+    //= aws-encryption-sdk-specification/framework/branch-key-store.md#aws-kms-branch-key-decryption
+    //= type=implication
+    //# - `GrantTokens` MUST be this keystore's [grant tokens](https://docs.aws.amazon.com/kms/latest/developerguide/concepts.html#grant_token).
+    && decryptRequest.GrantTokens == Some(grantTokens)
+
+    && decryptHistory.output.Success?
+    && decryptHistory.output.value.Plaintext.Some?
+
+  }
+
 
 }
